Fix semantics for interfaces; added careful semantics and automation for
underlying types and determining when a type is or is not an interface
type, which determines conversion semantics.

new/golang/defn/interface.v
@@ -6,16 +6,13 @@ Context {ext : ffi_syntax}.
 Context {go_lctx : GoLocalContext} {go_gctx : GoGlobalContext} `{!GoSemanticsFunctions}.
 
 Definition is_interface_type (t : go.type) : bool :=
-  match (to_underlying t) with
-  | go.InterfaceType _ => true
-  | _ => false
-  end.
+  match t with go.InterfaceType _ => true | _ => false end.
 
 (* Based on: https://go.dev/ref/spec#General_interfaces *)
 Definition type_set_term_contains {go_ctx : GoLocalContext} t (e : go.type_term) : bool :=
   match e with
   | go.TypeTerm t' => bool_decide (t = t')
-  | go.TypeTermUnderlying t' => bool_decide (to_underlying t = t')
+  | go.TypeTermUnderlying t' => bool_decide (underlying t = t')
   end.
 
 Definition type_set_elem_contains {go_ctx : GoLocalContext} t (e : go.interface_elem) : bool :=
@@ -29,42 +26,49 @@ Definition type_set_elems_contains {go_ctx : GoLocalContext} t (elems : list go.
 
 (** Equals [true] iff t is in the type set of t'. *)
 Definition type_set_contains {go_ctx : GoLocalContext} t t' : bool :=
-  match (to_underlying t') with
+  match (underlying t') with
   | go.InterfaceType elems => type_set_elems_contains t elems
   | _ => bool_decide (t = t')
   end.
 
 Class InterfaceSemantics :=
 {
+  #[global] convert_to_interface (v : val)
+    `{!from ↓u funder} `{!to ≤u go.InterfaceType elems} ::
+    go.GoExprEq (Convert from to v)
+      (Val (if is_interface_type funder then v else #(interface.mk from v)));
+
   #[global] interface_get_step m i ::
     go.IsGoStepPureDet (InterfaceGet m) #i
     (match i with
      | interface.nil => Panic "nil dereference in interface call"
      | interface.mk t v => (λ: "arg1", #(methods t m) v "arg1")%E
      end);
-  #[global] type_assert_step t i ::
+
+  #[global] type_assert_step `{!t ↓u tunder} i ::
     go.IsGoStepPureDet (TypeAssert t) #i
     (match i with
      | interface.nil => Panic "type assert failed"
      | interface.mk dt v =>
-         if is_interface_type t then
-           (if (type_set_contains dt t) then #i else Panic "type assert failed")
+         if is_interface_type tunder then
+           if (type_set_contains dt t) then #i else Panic "type assert failed"
          else
-           (if decide (t = dt) then v else Panic "type assert failed")
+           if decide (t = dt) then v else Panic "type assert failed"
      end);
-  #[global] type_assert2_step t i ::
+
+  #[global] type_assert2_interface_step `{!t ↓u tunder} i ::
     go.IsGoStepPureDet (TypeAssert2 t) #i
     (match i with
      | interface.nil => (#interface.nil, #false)%V
      | interface.mk dt v =>
-         if is_interface_type t then
-           (if (type_set_contains dt t) then (#i, #true)%V else (#interface.nil, #false)%V)
+         if is_interface_type tunder then
+           if (type_set_contains dt t) then (#i, #true)%V else (#interface.nil, #false)%V
          else
-           (if decide (t = dt) then (v, #true)%V else (GoZeroVal t #(), #false)%E)
+           if decide (t = dt) then (v, #true)%V else (GoZeroVal t #(), #false)%E
      end);
 
-  method_interface t m (H : is_interface_type t = true) :
-    #(methods t m) = (InterfaceGet m);
+  #[global] method_interface m `{!t ≤u go.InterfaceType elems} ::
+    go.GoExprEq #(methods t m) (InterfaceGet m);
 }.
 End defs.
 End go.
